examples/pseudo_bool/cp_encoding/README.md
@@ -3,8 +3,8 @@ CP semantics and encoders
 [cpScript.sml](cpScript.sml):
 Definition of CP problem syntax and semantics
 
-[cp_encodeScript.sml](cp_encodeScript.sml):
-Formalization of the CP encoder
+[cp_to_ilpScript.sml](cp_to_ilpScript.sml):
+Formalization of the CP to ILP phase
 
 [ilpScript.sml](ilpScript.sml):
 An ILP-style language designed as an intermediate layer for CP encodings
